src/arch/x64/X64.Vale.StrongPost_i.fst
@@ -22,30 +22,97 @@ let rec lemma_regs_match_self (regs:list reg) (s:state) : Lemma
   | [] -> ()
   | r::regs -> lemma_regs_match_self regs s
 
+let lemma_update_reg_equal (r:reg) (v:nat64) (s1:state) (s2:state) : Lemma
+  (requires (Regs_i.equal (update_reg r v s1).regs s2.regs))
+  (ensures ((update_reg r v s1).regs == s2.regs)) =
+  ()
+
+let lemma_strong_post_ins (i:ins) (inss:list ins) (s0:state) (sN:state) : Ghost (option state)
+  (requires
+    Some sN == va_eval_code (va_Block (inss_to_codes (i::inss))) s0 /\
+    s0.ok)
+  (ensures (fun sM ->
+    match sM with
+    | None -> strong_post (i::inss) s0 sN
+    | Some sM ->
+        Some sN == va_eval_code (va_Block (inss_to_codes inss)) sM /\
+        sM.ok /\
+        (strong_post inss sM sN ==> strong_post (i::inss) s0 sN))) =
+  let b0 = inss_to_codes (i::inss) in
+  let none_post () : Ghost (option state)
+    (requires normalize (strong_post (i::inss) s0 sN))
+    (ensures fun _ -> strong_post (i::inss) s0 sN) =
+    assert_norm (strong_post (i::inss) s0 sN);
+    None
+    in
+  let some_post_helper (sM:state) (p:Type0) : Ghost (option state)
+    (requires strong_post inss sM sN ==> normalize p)
+    (ensures fun _ -> strong_post inss sM sN ==> p) =
+    Some sM
+    in
+  let some_post (sM:state) : Ghost (option state)
+    (requires strong_post inss sM sN ==> normalize (strong_post (i::inss) s0 sN))
+    (ensures fun _ -> strong_post inss sM sN ==> strong_post (i::inss) s0 sN) =
+    some_post_helper sM (strong_post (i::inss) s0 sN)
+    in
+  match i with
+  | Mov64 (OReg dst) src ->
+      if dst <> Rsp && valid_operand_norm src s0 then
+        let (bM, sM) = va_lemma_Mov64 b0 s0 sN (OReg dst) src in
+        some_post sM
+      else none_post ()
+  | Load64 (OReg dst) (OReg src) offset ->
+      if dst <> Rsp && valid_src_addr s0.mem (s0.regs src + offset) then
+        let (bM, sM) = va_lemma_Load64 b0 s0 sN (OReg dst) (OReg src) offset in
+        some_post sM
+      else none_post ()
+  | Store64 (OReg dst) src offset ->
+      if valid_dst_addr s0.mem (s0.regs dst + offset) && valid_operand_norm src s0 then
+        let (bM, sM) = va_lemma_Store64 b0 s0 sN (OReg dst) src offset in
+        some_post sM
+      else none_post ()
+  | Add64Wrap (OReg dst) src ->
+      if dst <> Rsp && valid_operand_norm src s0 then
+        let (bM, sM) = va_lemma_Add64Wrap b0 s0 sN (OReg dst) src in
+        some_post sM
+      else none_post ()
+  | Adc64Wrap (OReg dst) src ->
+      if dst <> Rsp && valid_operand_norm src s0 then
+        let (bM, sM) = va_lemma_Adc64Wrap b0 s0 sN (OReg dst) src in
+        some_post sM
+      else none_post ()
+  | Mul64Wrap src ->
+      if valid_operand_norm src s0 then
+        let (bM, sM) = va_lemma_Mul64Wrap b0 s0 sN src in
+        some_post sM
+      else none_post ()
+  | IMul64 (OReg dst) src ->
+      let a = s0.regs dst `op_Multiply` eval_operand_norm src s0 in
+      if dst <> Rsp && valid_operand_norm src s0 && a < nat64_max then
+        let (bM, sM) = va_lemma_IMul64 b0 s0 sN (OReg dst) src in
+        some_post sM
+      else none_post ()
+  | _ -> assume false; None
+
 let rec lemma_strong_post (inss:list ins) (s0:state) (sN:state) : Lemma
   (requires
     Some sN == va_eval_code (va_Block (inss_to_codes inss)) s0 /\
     s0.ok)
   (ensures
     strong_post inss s0 sN) =
-  let b0 = inss_to_codes inss in
   match inss with
   | [] ->
       let _ = va_lemma_empty s0 sN in
       let regs = [Rax; Rbx; Rcx; Rdx; Rsi; Rdi; Rbp; Rsp; R8; R9; R10; R11; R12; R13; R14; R15] in
       lemma_regs_match_self regs s0;
+      assert_norm (strong_post inss s0 sN);
       ()
-  | (Load64 (OReg dst) (OReg src) offset)::inss ->
-      if dst <> Rsp && valid_src_addr s0.mem (s0.regs src + offset) then
-        let (bM, sM) = va_lemma_Load64 b0 s0 sN (OReg dst) (OReg src) offset in
-        lemma_strong_post inss sM sN
-      else ()
-  | (Store64 (OReg dst) (OReg src) offset)::inss ->
-      if valid_dst_addr s0.mem (s0.regs dst + offset) then
-        let (bM, sM) = va_lemma_Store64 b0 s0 sN (OReg dst) (OReg src) offset in
-        lemma_strong_post inss sM sN
-      else ()
-  | _ -> ()
+  | i::inss ->
+    (
+      match lemma_strong_post_ins i inss s0 sN with
+      | None -> ()
+      | Some sM -> lemma_strong_post inss sM sN
+    )
 
 let assert_to_norm (p:Type0) : Lemma
   (requires p)
