src/arch/x64/X64.Vale.StrongPost_i.fsti
@@ -20,12 +20,38 @@ val lemma_mem_upd : m:mem -> i:int -> n:nat64 -> Lemma
   [SMTPat (mem_upd m i n)]
 
 type ins =
+  | Mov64 : dst:va_operand -> src:va_operand -> ins
   | Load64 : dst:va_operand -> src:va_operand -> offset:int -> ins
   | Store64 : dst:va_operand -> src:va_operand -> offset:int -> ins
+  | Add64Wrap : dst:va_operand -> src:va_operand -> ins
+  | Adc64Wrap : dst:va_operand -> src:va_operand -> ins
+  | Mul64Wrap : src:va_operand -> ins
+  | IMul64 : dst:va_operand -> src:va_operand -> ins
 
-unfold let va_inss = list ins
+unfold let va_fast_ins_Mov64 = Mov64
 unfold let va_fast_ins_Load64 = Load64
 unfold let va_fast_ins_Store64 = Store64
+unfold let va_fast_ins_Add64Wrap = Add64Wrap
+unfold let va_fast_ins_Adc64Wrap = Adc64Wrap
+unfold let va_fast_ins_Mul64Wrap = Mul64Wrap
+unfold let va_fast_ins_IMul64 = IMul64
+
+unfold let va_inss = list ins
+
+let valid_maddr_norm (m:maddr) (s:state) : bool =
+  mem_contains s.mem (eval_maddr m s)
+
+let valid_operand_norm (o:operand) (s:state) : bool =
+  match o with
+  | OConst n -> 0 <= n && n < nat64_max
+  | OReg r -> true
+  | OMem m -> valid_maddr_norm m s
+
+let eval_operand_norm (o:operand) (s:state) : nat64 =
+  match o with
+  | OConst n -> if 0 <= n && n < nat64_max then n else 0
+  | OReg r -> s.regs r
+  | OMem m -> mem_sel s.mem (eval_maddr m s)
 
 let rec regs_match (regs:list reg) (s0:state) (s1:state) =
   match regs with
@@ -36,6 +62,7 @@ let all_regs_match (s0:state) (s1:state) =
   let regs = [Rax; Rbx; Rcx; Rdx; Rsi; Rdi; Rbp; Rsp; R8; R9; R10; R11; R12; R13; R14; R15] in
   regs_match regs s0 s1
 
+[@"opaque_to_smt"] // because of exists-interp axiom, avoid giving this to SMT
 let rec strong_post (inss:list ins) (s0:state) (sN:state) : Type0 =
   match inss with
   | [] ->
@@ -43,24 +70,69 @@ let rec strong_post (inss:list ins) (s0:state) (sN:state) : Type0 =
       sN.flags == s0.flags /\
       sN.mem == s0.mem /\
       all_regs_match s0 sN // for efficiency, we apply s0.regs to all registers and then discard s0.regs
-  | (Load64 (OReg Rsp) (OReg src) offset)::inss -> True
+  | (Mov64 (OReg Rsp) _)::_ -> True
+  | (Mov64 (OReg dst) src)::inss ->
+      not (valid_operand_norm src s0) \/
+      (exists x.
+        x == eval_operand_norm src s0 /\
+        strong_post inss (update_reg dst x s0) sN)
+  | (Load64 (OReg Rsp) _ _)::_ -> True
   | (Load64 (OReg dst) (OReg src) offset)::inss ->
       not (mem_contains s0.mem (s0.regs src + offset)) \/
       (exists x.
         x == mem_sel s0.mem (s0.regs src + offset) /\
         strong_post inss (update_reg dst x s0) sN)
-  | (Store64 (OReg dst) (OReg src) offset)::inss ->
+  | (Store64 (OReg dst) src offset)::inss ->
+      not (valid_operand_norm src s0) \/
       not (mem_contains s0.mem (s0.regs dst + offset)) \/
       (exists x.
-        x == mem_upd s0.mem (s0.regs dst + offset) (s0.regs src) /\
+        x == mem_upd s0.mem (s0.regs dst + offset) (eval_operand_norm src s0) /\
         strong_post inss ({s0 with mem = x}) sN)
+  | (Add64Wrap (OReg Rsp) _)::_ -> True
+  | (Add64Wrap (OReg dst) src)::inss ->
+      not (valid_operand_norm src s0) \/
+      (exists a x (f:nat64).
+        a == s0.regs dst + eval_operand_norm src s0 /\
+        x == (if a < nat64_max then a else a - nat64_max) /\
+        cf f == (a >= nat64_max) /\
+        strong_post inss ({update_reg dst x s0 with flags = f}) sN)
+  | (Adc64Wrap (OReg Rsp) _)::_ -> True
+  | (Adc64Wrap (OReg dst) src)::inss ->
+      not (valid_operand_norm src s0) \/
+      (exists a x (f:nat64).
+        a == s0.regs dst + eval_operand_norm src s0 + (if cf s0.flags then 1 else 0) /\
+        x == (if a < nat64_max then a else a - nat64_max) /\
+        cf f == (a >= nat64_max) /\
+        strong_post inss ({update_reg dst x s0 with flags = f}) sN)
+  | (Mul64Wrap src)::inss ->
+      not (valid_operand_norm src s0) \/
+      (exists (rax:nat64) (rdx:nat64) (f:nat64).
+        nat64_max `op_Multiply` rdx + rax == s0.regs Rax `op_Multiply` eval_operand_norm src s0 /\
+        strong_post inss (update_reg Rdx rdx (update_reg Rax rax ({s0 with flags = f}))) sN)
+  | (IMul64 (OReg Rsp) _)::_ -> True
+  | (IMul64 (OReg dst) src)::inss ->
+      let a = s0.regs dst `op_Multiply` eval_operand_norm src s0 in
+      not (valid_operand_norm src s0) \/
+      not (a < nat64_max) \/
+      (exists (x:nat64) (f:nat64).
+        x == a /\
+        strong_post inss ({update_reg dst x s0 with flags = f}) sN)
   | _ -> True
 
 let rec inss_to_codes (inss:list ins) : list va_code =
   match inss with
-  | (Load64 (OReg Rsp) (OReg src) offset)::inss -> []
+  | (Mov64 (OReg Rsp) _)::inss -> []
+  | (Mov64 (OReg dst) src)::inss -> (va_code_Mov64 (OReg dst) src)::(inss_to_codes inss)
+  | (Load64 (OReg Rsp) _ _)::inss -> []
   | (Load64 (OReg dst) (OReg src) offset)::inss -> (va_code_Load64 (OReg dst) (OReg src) offset)::(inss_to_codes inss)
-  | (Store64 (OReg dst) (OReg src) offset)::inss -> (va_code_Store64 (OReg dst) (OReg src) offset)::(inss_to_codes inss)
+  | (Store64 (OReg dst) src offset)::inss -> (va_code_Store64 (OReg dst) src offset)::(inss_to_codes inss)
+  | (Add64Wrap (OReg Rsp) _)::inss -> []
+  | (Add64Wrap (OReg dst) src)::inss -> (va_code_Add64Wrap (OReg dst) src)::(inss_to_codes inss)
+  | (Adc64Wrap (OReg Rsp) _)::inss -> []
+  | (Adc64Wrap (OReg dst) src)::inss -> (va_code_Adc64Wrap (OReg dst) src)::(inss_to_codes inss)
+  | (Mul64Wrap src)::inss -> (va_code_Mul64Wrap src)::(inss_to_codes inss)
+  | (IMul64 (OReg Rsp) _)::inss -> []
+  | (IMul64 (OReg dst) src)::inss -> (va_code_IMul64 (OReg dst) src)::(inss_to_codes inss)
   | _ -> []
 
 val va_lemma_strong_post_norm : inss:list ins -> s0:state -> sN:state -> Lemma
